# 1. Given an array, return the indices of the two numbers such that they add up to the target https://leetcode.com/problems/two-sum/

- Using hash table (HashMap in Java, Dict in Python): O(n) & S(n)

Java:

```java
class Solution {
    public int[] twoSum(int[] nums, int target) {
        HashMap<Integer, Integer> Indices = new HashMap<Integer, Integer>();
        for (int i=0; i<nums.length; i++) {
            if (Indices.containsKey(target-nums[i]))
                return new int[]{i, Indices.get(target-nums[i])};
            else
                Indices.put(nums[i], i);
        }
        return new int[2];
    }
}
```

Python:

```python
class Solution:
    def twoSum(self, nums: List[int], target: int) -> List[int]:
        index_dict={}
        for i in range(len(nums)):
            if index_dict.get(target-nums[i]) is not None:
                return [i, index_dict.get(target-nums[i])]
            index_dict[nums[i]] = i
```

# 2. Given two sorted array, merge them into single sorted array and done in-place. https://leetcode.com/problems/merge-sorted-array/

- Use two pointers from back to front: O(m+n) & S(1)

Java:

```java 
class Solution {
    public void merge(int[] nums1, int m, int[] nums2, int n) {
        int i = m-1;
        int j = n-1;
        int k = i+j+1;
            
        while (i>=0 && j>=0){
            if (nums2[j] >= nums1[i]){
                nums1[k] = nums2[j];
                k--;
                j--;
            }
            else{
                nums1[k] = nums1[i];
                k--;
                i--;
            }
        }
        while (j>=0){
            nums1[j] = nums2[j];
            j--;
        }
    }
}
```

Python:

```python
class Solution:
    def merge(self, nums1: List[int], m: int, nums2: List[int], n: int) -> None:
        """
        Do not return anything, modify nums1 in-place instead.
        """
        while m > 0 and n > 0:
            if nums1[m-1] > nums2[n-1]:
                nums1[m+n-1] = nums1[m-1]
                m -= 1
            else:
                nums1[m+n-1] = nums2[n-1]
                n -= 1
        nums1[:n] = nums2[:n]
        
```
